chore: all proofs

RISCV/SailPure.lean
@@ -33,13 +33,7 @@ def shiftiwop (shamt : BitVec 5) (op : sopw) (rs1_val : BitVec 64) : BitVec 64 :
     | sopw.SRAIW => (shift_bits_right_arith rs1_val32 shamt)
   (sign_extend (m := ((2 ^i 3) *i 8)) result)
 
-def shiftiop (shamt : BitVec 6) (op : sop) (rs1_val : BitVec 64) : BitVec 64 :=
-  match op with
-  | sop.SLLI => (Sail.shift_bits_left rs1_val shamt)
-  | sop.SRLI => (Sail.shift_bits_right rs1_val shamt)
-  | sop.SRAI => (shift_bits_right_arith rs1_val shamt)
-
-def rtipew (op : ropw) (rs2_val : BitVec 64) (rs1_val : BitVec 64) : BitVec 64 :=
+def rtypew (op : ropw) (rs2_val : BitVec 64) (rs1_val : BitVec 64) : BitVec 64 :=
   let rs1_val32 := Sail.BitVec.extractLsb rs1_val 31 0
   let rs2_val32 :=  Sail.BitVec.extractLsb rs2_val 31 0
   let result : (BitVec 32) :=
